theories/L1g/toplevel.v
@@ -4,10 +4,10 @@ Require Import L1g.program.
 Require Import L1g.wcbvEval.
 Require Import Common.Common Common.classes Common.Pipeline_utils Common.compM.
 From ExtLib Require Import Monads.
-
+From MetaCoq.Template Require Import utils Typing.
 Import MonadNotation.
 
-Definition erase_PCUIC : CertiCoqTrans Ast.program (global_context * term) :=
+Definition erase_PCUIC : CertiCoqTrans Ast.Env.program (global_context * term) :=
   fun src =>
     debug_msg "Translating from Template to Lbox" ;;
     (LiftErrorCertiCoqTrans "Lbox" L1g.compile.erase src).
@@ -18,13 +18,21 @@ Definition compile_L1g : CertiCoqTrans (global_context * term) (Program Term) :=
     debug_msg "Translating from Lbox to L1" ;;
     (LiftCertiCoqTrans "L1g" L1g.compile.program_Program src).
 
-(* Zoe: AFAICT we don't have these definitions *)
-(* Instance Template_Lang : Lang Ast.program := *)
-(*   { Value := Ast.term; *)
-(*     TermWf := _ ; *)
-(*     BigStep := _ }. *)
+Definition wf_program (p : Ast.Env.program) := 
+  ∥ ∑ T, @Typing.typing 
+    config.extraction_checker_flags
+    (Ast.Env.empty_ext p.1)
+    [] p.2 T ∥.
 
-Instance L1g_Lang : Lang (Program Term) :=
+Definition template_bigstep (p : Ast.Env.program) (v : Ast.term) : Prop :=
+  ∥ Template.WcbvEval.eval p.1 [] p.2 v ∥.
+
+#[export] Instance Template_Lang : Lang Ast.Env.program :=
+  { Value := Ast.term;
+    TermWf := wf_program ;
+    BigStep := template_bigstep }.
+
+#[global] Instance L1g_Lang : Lang (Program Term) :=
   { Value := Term;
     TermWf := fun P => match P with
                       mkPgm trm env => WFapp trm /\ program.WFaEnv env
